yes good

2.dfy
@@ -2,28 +2,48 @@
 
 /*
     Daniel Cavalheiro   57869
-    Perdro Nunes        57854
+    Pedro Nunes        57854
 */
 
 datatype List<T> = Nil | Cons(head: T, tail: List<T>)
 
-function lenght<T>(l: List<T>): nat 
+function length<T>(l: List<T>): nat
 {
-    match l
-        case Nil => 0
-        case Cons(_, t) => 1 + lenght(t)
+  match l
+  case Nil => 0
+  case Cons(_, t) => 1 + length(t)
+}
+
+function mem<T(==)> (x: T, l: List<T>) : bool
+{
+  match l
+  case Nil => false
+  case Cons(head, t) => if(head == x)
+  then true
+  else
+    mem(x,t)
 }
 
 
 method from_array<T>(a: array<T>) returns (l: List<T>)
-    requires a.Length >= 0
-    ensures lenght(l) == a.Length
+  requires a.Length >= 0
+  ensures length(l) == a.Length
+  ensures forall i: int :: 0 <= i < a.Length ==> mem(a[i], l)
+
 {
-    l := Nil;
-    var i: int := a.Length-1;
-    while(i >= 0)
-    {
-        l := Cons(a[i], l);
-        i := i-1;
-    }
-} 
+  l := Nil;
+  var i: int := a.Length - 1;
+  while(i >= 0)
+    invariant -1 <= i <= a.Length - 1
+    invariant forall j: int ::  i < j <= a.Length - 1 ==> mem(a[j], l)
+    invariant length(l) == a.Length - 1 - i
+  {
+    l := Cons(a[i], l);
+    i := i-1;
+  }
+}
+
+method main() {
+  var l: List<int> := Cons(1, Nil);
+  assert length(l) == 1;
+}
